# Solving Quadratic Equations by Completing the Square

## A Quick Reminder: Special Products ðŸ’¡

Before we begin, let's remember three key algebraic identities. Recognizing these patterns is a useful shortcut.

* **Square of a Sum:**
  $(a+b)^2 = a^2 + 2ab + b^2$

* **Square of a Difference:**
  $(a-b)^2 = a^2 - 2ab + b^2$

* **Difference of Squares:**
  $(a+b)(a-b) = a^2 - b^2$

---

## The Goal: Creating a Perfect Square

As we saw in the special products, a perfect square trinomial is what you get when you square a binomial. For example:
$x^2 + 10x + 25 = (x+5)^2$

The method of **"completing the square"** is a technique to turn one side of a quadratic equation into one of these perfect square trinomials. We do this by finding the one "missing" number that completes the pattern.

The name comes from the geometric idea of having an incomplete square and finding the small corner piece needed to finish it.

---

## Worked Example #1

Solve:
$x^2 + 6x - 16 = 0$

**1. Isolate the x-terms:**
$x^2 + 6x = 16$

**2. Complete the square:**
Take half of 6 â†’ 3, square it â†’ 9. Add to both sides.
$x^2 + 6x + 9 = 16 + 9$

**3. Factor the perfect square:**
$(x+3)^2 = 25$

**4. Take the square root:**
$x+3 = \pm5$

**5. Solve for x:**

* $x+3 = 5 \Rightarrow x = 2$
* $x+3 = -5 \Rightarrow x = -8$

âœ… **Solutions:** $x=2$, $x=-8$

---

## Worked Example #2 (with a different sign)

Solve:
$x^2 - 10x + 1 = 0$

**1. Isolate the x-terms:**
$x^2 - 10x = -1$

**2. Complete the square:**
Take half of -10 â†’ -5, square it â†’ 25. Add to both sides.
$x^2 - 10x + 25 = -1 + 25$

**3. Factor the perfect square:**
$(x-5)^2 = 24$

**4. Take the square root:**
$x-5 = \pm\sqrt{24}$
Simplify: $\sqrt{24} = 2\sqrt{6}$
$x - 5 = \pm 2\sqrt{6}$

**5. Solve for x:**
$x = 5 \pm 2\sqrt{6}$

âœ… **Solutions:** $x = 5 + 2\sqrt{6}$, $x = 5 - 2\sqrt{6}$

---

## Worked Example #3 (with an odd middle term)

Solve:
$x^2 + 3x - 4 = 0$

**1. Isolate the x-terms:**
$x^2 + 3x = 4$

**2. Complete the square:**
Take half of 3 â†’ $\tfrac{3}{2}$, square it â†’ $\tfrac{9}{4}$. Add to both sides.
$x^2 + 3x + \tfrac{9}{4} = 4 + \tfrac{9}{4}$

**3. Factor the perfect square:**
$(x+\tfrac{3}{2})^2 = \tfrac{16}{4} + \tfrac{9}{4} = \tfrac{25}{4}$

**4. Take the square root:**
$x + \tfrac{3}{2} = \pm\sqrt{\tfrac{25}{4}} = \pm\tfrac{5}{2}$

**5. Solve for x:**

* $x + \tfrac{3}{2} = \tfrac{5}{2} \Rightarrow x = 1$
* $x + \tfrac{3}{2} = -\tfrac{5}{2} \Rightarrow x = -4$

âœ… **Solutions:** $x=1$, $x=-4$

---

## Steps to Follow for Completing the Square

1. **Standard Form:** Write in $ax^2 + bx + c = 0$. If $a \neq 1$, divide everything by $a$.
2. **Isolate:** Move the constant term $c$ to the other side.
3. **Find the "Magic Number":** Take $b$, divide by 2, square it â†’ $(\tfrac{b}{2})^2$.
4. **Add to Both Sides:** Keep the equation balanced.
5. **Factor:** Left side becomes a perfect square trinomial â†’ $(x+\tfrac{b}{2})^2$.
6. **Take the Square Root:** Remember $\pm$ on the right.
7. **Solve for x:** Isolate x.

---

## When to Use Completing the Square

* **Deriving the Quadratic Formula**: This is the foundation.
* **When Factoring Doesnâ€™t Work**: A reliable fallback.
* **Graphing Circles & Conics**: Essential for standard forms.
* **When $a=1$ and $b$ is even**: Especially quick, avoids fractions.
